# Deriving multipliers and calculating the multiplier effects

- [The default formula](#the-default-formula)
- [Types of variables](#types-of-variables)
  - [1. Exogenous variables (predetermined/given)](#1-exogenous-variables-predeterminedgiven)
  - [2. Endogenous variables (determined by the model)](#2-endogenous-variables-determined-by-the-model)
- [Multipliers and their effects](#multipliers-and-their-effects)
- [Steps for the model](#steps-for-the-model)
- [Steps for the multiplier effects](#steps-for-the-multiplier-effects)
  - [**1. Variation in output**](#1-variation-in-output)
  - [**2. Variation in disposable income**](#2-variation-in-disposable-income)
  - [**3. Variation in budget deficit**](#3-variation-in-budget-deficit)

<ins>[**Seminar PDF 1**](./seminar%20pdfs/S04.%20Deriving%20multipliers%20and%20calculating%20the%20multiplier%20effects%20(1).pdf)  
<ins>[**Seminar PDF 2**](./seminar%20pdfs/S04.%20Deriving%20multipliers%20and%20calculating%20the%20multiplier%20effects%20(2).pdf)

---

## <ins>The default formula
Consider the case of a close economy:  
$y = C + I + G$
> $y$ - GDP in market prices  
> $C$ - consumption  
> $C = C_0 + c \cdot y^D$  
>> $C_0$ - autonomous consumption (expenditure made for goods and services that cover basic needs)  
>> $c$ - marginal propensity to consume, $c = \dfrac{\Delta c}{\Delta y^D}$  
>> $y^D$ - disposable income, $y^D = y - T + Tr$  
>>> $Tr$ - transfers  
>>> $T$ - taxes, $T = T_0 + t \cdot y$  
>>> t - tax rate  
>>> $T_0$ - autonomous tax  

---

## <ins>Types of variables
### 1. Exogenous variables (predetermined/given)
   - $I$, $G$, $Tr$, $C_0$, $T_0$  
### 2. Endogenous variables (determined by the model)
   - $y$, $c$, $y^D$, $T$  

---

## Multipliers and their effects
- A multiplier shows the impact of a change in 1 variable (that is exogenous) on another variable (that is endogenous) $\Rightarrow$ a formula  
- The multiplier effect shows the change $\Rightarrow$ a value that we calculate using the formula defined prior

---

## Steps for the model  
We write the <ins>reduced</ins> form of the model:  
$y = C_0 + c \cdot (y - T_0 - t \cdot y + Tr) + I + G$  
$y = C_0 - c \cdot T_0 + c \cdot Tr + I + G + c \cdot (1 - t) \cdot y$  
$(1 - c \cdot (1 - t)) \cdot y = C_0 - c \cdot T_0 + c \cdot Tr + I + G$  
$y = \dfrac{1}{1 - c \cdot (1 - t)} \cdot (C_0 - c \cdot T_0 + C \cdot Tr + I + G)$ **(reduced form of the model)**  

---

## Steps for the multiplier effects

> You can also find the official solutions on the <ins>[**Solution PDF**](./seminar%20pdfs/S04.%20Solutions.pdf)

Now we use these 4 equations:  

$$\begin{cases}
    y = C + I + G\\
    C = C_0 + c \cdot y^D\\
    y^D = y - T + Tr\\
    T = T_0 + t \cdot y\\
\end{cases}$$

to determine what changes in the reduced form of the model  

---

### **1. Variation in output**  
1. assume a change in <ins>government spending</ins> $G$  
    $\Delta y = \dfrac{1}{1 - c \cdot (1 - t)} \cdot \Delta G$  
    $\alpha _G = \dfrac{\Delta y}{\Delta G} = \dfrac{1}{1 - c \cdot (1 - t)} \Rightarrow$ **government spending multiplier**  

2. assume a change in <ins>investment</ins> $I$  
    $\Delta y = \dfrac{1}{1 - c \cdot (1 - t)} \cdot \Delta I \Rightarrow \alpha _I = \dfrac{\Delta y}{\Delta I} = \alpha _G \Rightarrow$ **investment multiplier**  

3. assume a change in <ins>autonomous consumption</ins> $C_0$  
    $\Delta y = \dfrac{1}{1 - c \cdot (1 - t)} \cdot \Delta C_0$  
    $\alpha _{C _0} = \dfrac{\Delta y}{\Delta C _0} = \alpha _g \Rightarrow$ **autonomous consumption multiplier**  

4. assume a change in <ins>autonomous taxes</ins> $T_0$  
    $\Delta y = \dfrac{1}{1 - c \cdot (1 - t)} \cdot (-c) \cdot \Delta T_0$  
    $\alpha _{T _0} = \dfrac{\Delta y}{\Delta T _0} = (-c) \cdot \alpha _G \Rightarrow$ **autonomous tax multiplier**  

5. assume a change in <ins>transfers</ins> $Tr$  
    $\Delta y = \dfrac{1}{1 - c \cdot (1 - t)} \cdot c \cdot \Delta Tr$  
    $\alpha _{Tr} = \dfrac{\Delta y}{\Delta Tr} = C \cdot \alpha _G \Rightarrow$ **transfers multiplier**  

6. assume a change in the <ins>tax rate</ins> $t$ 
    $y_1 = \dfrac{1}{1 - c \cdot (1 - t _1)} \cdot ()$  
    $y_0 = \dfrac{1}{1 - c \cdot (1 - t _0)} \cdot ()$  
    $\Delta y = y _1 - y _0 = \dfrac{1}{1 - c \cdot (1 - t _1)} \cdot () - \dfrac{1}{1 - c \cdot (1 - t _0)} \cdot ()$  
    > Actually $\dfrac{1}{1 - c \cdot (1 - t _0)} \cdot ()$ is $y _0 \Rightarrow$  

    $\Delta y = \dfrac{1 - c \cdot (1 - t _0) - 1 + c \cdot (1 - t _1)}{(1 - c \cdot(1 - t _1)) \cdot (1 - c \cdot(1 - t _0))}$  
    $\Delta y = \dfrac{(-c) \cdot t _1 + c \cdot t _0}{1 - c \cdot (1 - t _1)} \cdot y_0$  
    $\Delta y = \dfrac{(-c) \cdot \Delta t}{1 - c \cdot (1 - t _1)} \cdot y_0$  
    $\Rightarrow \alpha _t = \dfrac{\Delta y}{\Delta t} = \dfrac{(-c) \cdot y _0}{1 - c \cdot (1 - t _1)} \Rightarrow$ **tax rate multiplier**  
    > In some textbooks we find $\alpha _t = \dfrac{-c \cdot y _0}{1 - c(1 - t_0)}$ (because the difference is not too big)  
    > also we will get this formula at the exam in order to not waste time with deriving the formula in the way we did above

---

### **2. Variation in disposable income**  
the extended formula for $y^D$  
$y^D = y - T_0 - t \cdot y + Tr$  
$y^D = (1 - t) \cdot y - T _0 + Tr$ **(extended formula)**  
$y^D = (1 - t) \cdot \Delta y - \Delta T _0 + \Delta Tr$ **(variation of extended formula)**  

1. assume a change in <ins>government spending</ins> $G$  
    $\Delta y^D = (1 - t) \cdot \Delta y$  
    $\Delta y^D = (1 - t)$  
    $\dfrac{\Delta y}{\Delta G} = \alpha _G \Rightarrow \Delta y = \alpha _G \cdot \Delta G$  
    $\Rightarrow m \cdot \Delta y ^D _G = \dfrac{\Delta y^D}{\Delta G} = (1 - t) \cdot \alpha _G$  
    > m - multiplier  

2. assume a change in <ins>investment</ins> $I$  
    $\Delta y^D = (1 - t) \cdot \Delta y$  
    $\Delta y^D = (1 - t) \cdot \alpha _I \cdot \Delta I$  
    $\Rightarrow m \cdot \Delta y ^D _G = \dfrac{\Delta y^D}{\Delta I} = (1 - t) \cdot \alpha _G$  
    > We know that $\alpha _I = \alpha _G$  

3. assume a change in <ins>transfers</ins> $Tr$
    $\Delta y^D = (1 - t) \cdot \Delta y + \Delta Tr$  
    > we know from **government spending multiplier** that $\Delta y^D = \dfrac{1}{1 - c \cdot (1 - t)} \cdot c \cdot \Delta Tr$

    $\Rightarrow \Delta y^D = \dfrac{(1 - t) \cdot c \cdot \Delta Tr}{1 - c(1 - t)} + \Delta Tr$  
    $\Delta y^D = \dfrac{(1 - t) \cdot c \cdot \Delta Tr + (1 - c \cdot (1 - t)) \cdot \Delta Tr}{1 - c \cdot (1 - t)}$  
    $\Delta y^D = \dfrac{\Delta Tr((1 - t) \cdot c + 1 - c \cdot (1 - t))}{1 - c \cdot (1 - t)}$  
    $\Delta y^D = \dfrac{\Delta Tr}{1 - c \cdot (1 - t)} = \Delta Tr \cdot \alpha _G$  
    $\Rightarrow m \cdot \Delta y ^D _Tr = \dfrac{\Delta y^D}{\Delta Tr} = \alpha _G$  

4. assume a change in <ins>autonomous taxes</ins> $T_0$  
    $\Delta y^D = (1 - t) \cdot \Delta y - \Delta T _0$  
    > we know from **autonomous tax multiplier** that $\Delta y = (-c) \cdot \alpha \cdot \Delta T$  
    
    $\Delta y^D = (1 - t)((-c) \cdot \alpha _G \cdot \Delta T _0) - \Delta T _0$  
    $\Delta y^D = \left(\dfrac{(-c) \cdot (1 - t)}{1 - c \cdot (1 - t)} - 1 \right) \cdot \Delta T_0$  
    $\Delta y^D = \dfrac{(-c) \cdot (1 - t) - 1 + c \cdot (1 - t)}{1 - c \cdot (1-t)} \cdot \Delta T_0$  
    $\Delta y^D = -\alpha _G \cdot \Delta T _0$  
    $\Rightarrow m \cdot \Delta y^D _{T _0} = \dfrac{\Delta y^D}{\Delta T _0} = - \alpha _G$  

5. assume a change in tax rate $t$  
    $y ^D _1 = (1 - t_1) \cdot y _1 - T _0 + Tr$  
    $y ^D _0 = (1 - t_0) \cdot y _0 - T _0 + Tr$  
    $\Delta y^D = y ^D _1 - y ^D _0 = (1 - t_1) \cdot y _1 - (1 - t_0) \cdot y_0$  
    $\Delta y^D = y _1 - t _1 \cdot y_1 - y _0 + t _0 \cdot y _0$  
    $\Delta y^D = \Delta y - t _1 \cdot y_1 + t _0 \cdot y _0$  
    > Note: $y _1 \cdot \Delta t - t _0 \cdot \Delta y = t _1 \cdot y _1 + t _0 \cdot y _0$, thus $\Delta y^D = \Delta y + y _1 \cdot \Delta t - t_0 \cdot \Delta y$  

    $\Delta y^D = (1 - t _0) \cdot \Delta y + y _1 \cdot \Delta t$  
    $\Delta y^D = \dfrac{(-c) \cdot \Delta t}{1 - c \cdot (1 - t _1)}$  
    $\Delta y^D = (1 - t_0) \left(\dfrac{(-c) \cdot \Delta t}{1 - c \cdot (1 - t _1)} \right) + y _1 \cdot \Delta t$  
    $m \cdot \Delta y ^D _t = \dfrac{\Delta y^D}{\Delta t} = \dfrac{(-c) \cdot (1 - t _0)}{1 - c \cdot (1 - t _1)} + y _1$  

### **3. Variation in budget deficit**  

$BD = G - T + Tr + Sv$  
$\Delta BD = \Delta G - \Delta T + \Delta Tr + \Delta Sv$  
$T = T _0 + t \cdot y$  
$\Delta T = \Delta T _0 + t \cdot \Delta y$ (except for changes in t)  

1. assume a change in <ins>government spending</ins> $G$  
    $\Delta BD = \Delta G - \Delta T _0 - t \cdot \Delta y + \Delta Tr + \Delta Sv$  
    $\Delta BD = \Delta G - t \cdot \Delta y$  
    $\Delta y = \alpha _G \cdot \Delta G$  
    $\Delta BD = \Delta G - t \cdot \alpha _G \cdot \Delta G$  
    $\Delta BD = (1 - t \cdot \alpha _G) \cdot \Delta G$  
    $m \cdot BD _G = \dfrac{\Delta BD}{\Delta G} = 1 - t \cdot \alpha _G$  

2. assume a change in <ins>transfers</ins> $Tr$  
    $\Delta BD = \Delta G - \Delta T _0 - t \cdot \Delta y + \Delta Tr + \Delta Sv$  
    $\Delta BD = (-t) \cdot \Delta y + \Delta Tr$  
    $\Delta y = c \cdot \alpha _G \cdot\Delta Tr$  
    $\Delta BD = (-t) \cdot c \cdot \alpha _G \cdot \Delta Tr + \Delta Tr$  
    $m \cdot BD _{Tr} = \dfrac{\Delta BD}{\Delta Tr} = 1 - t \cdot c \cdot \alpha _G$  
